books/data/treeset/diff.lisp
@@ -12,25 +12,55 @@
 (include-book "std/util/defrule" :dir :system)
 (include-book "xdoc/constructors" :dir :system)
 
+(include-book "data/utilities/oset-defs" :dir :system)
+
 (include-book "internal/tree-defs")
 (include-book "internal/diff-defs")
 (include-book "set-defs")
 (include-book "in-defs")
 (include-book "subset-defs")
+(include-book "insert-defs")
 (include-book "union-defs")
+(include-book "to-oset-defs")
 
 (local (include-book "std/basic/controlled-configuration" :dir :system))
 (local (acl2::controlled-configuration :hooks nil))
 
+(local (include-book "std/osets/top" :dir :system))
+
 (local (include-book "internal/tree"))
 (local (include-book "internal/in"))
 (local (include-book "internal/diff"))
+(local (include-book "internal/in-order"))
 (local (include-book "set"))
 (local (include-book "cardinality"))
 (local (include-book "in"))
 (local (include-book "insert"))
 (local (include-book "subset"))
 (local (include-book "union"))
+(local (include-book "to-oset"))
+
+;;;;;;;;;;;;;;;;;;;;;;;;;;;;;;;;;;;;;;;;;;;;;;;;;;;;;;;;;;;;;;;;;;;;;;;;;;;;;;;;
+
+(defxdoc diff
+  :parents (treeset)
+  :short "Set difference on @(see treeset)s."
+  :long
+  (xdoc::topstring
+    (xdoc::p
+      "Time complexity: @($O(n\\log(m/n))$) (where @($n < m$)).")
+    (xdoc::section
+      "General form"
+      (xdoc::codeblock
+        "(diff x y :test test)")
+      (xdoc::desc
+        "@(':test') &mdash; optional"
+        (xdoc::p
+          "One of: @('equal'), @('='), @('eq'), or @('eql'). If no value is
+           provided, the default is @('equal'). Specifying an alternative test
+           allows for a more performant implementation, at the cost of a
+           stronger guard. The guard asserts that the set consists of elements
+           suitable for comparison with the specified equality variant.")))))
 
 ;;;;;;;;;;;;;;;;;;;;;;;;;;;;;;;;;;;;;;;;;;;;;;;;;;;;;;;;;;;;;;;;;;;;;;;;;;;;;;;;
 
@@ -44,22 +74,15 @@
 
 ;;;;;;;;;;;;;;;;;;;;;;;;;;;;;;;;;;;;;;;;
 
-;; TODO: doc should be on diff
 (define diff$inline
   ((x setp)
    (y setp))
-  :parents (set)
-  :short "Set difference."
-  :long
-  (xdoc::topstring
-    (xdoc::p
-      "Time complexity: @($O(n\\log(m/n))$) (where @($n < m$))."))
   :returns (set setp
                 :hints (("Goal" :in-theory (enable setp
                                                    fix
                                                    empty))))
   (tree-diff (fix x) (fix y))
-  :guard-hints (("Goal" :in-theory (enable setp)))
+  :guard-hints (("Goal" :in-theory (enable* break-abstraction)))
 
   ///
   (add-macro-fn diff diff$inline))
@@ -68,10 +91,18 @@
 
 (in-theory (disable (:t diff)))
 
+(defruled diff-type-prescription
+  (or (consp (diff x y))
+      (equal (diff x y) nil))
+  :rule-classes :type-prescription
+  :enable diff)
+
+(add-to-ruleset break-abstraction '(diff-type-prescription))
+
 (defrule diff-when-equiv-of-arg1-congruence
   (implies (equiv x0 x1)
-           (equal (diff x0 z)
-                  (diff x1 z)))
+           (equal (diff x0 y)
+                  (diff x1 y)))
   :rule-classes :congruence
   :enable diff)
 
@@ -129,6 +160,44 @@
   :enable (double-containment
            pick-a-point))
 
+;;;;;;;;;;;;;;;;;;;;
+
+(defrule oset-difference-of-to-oset
+  (equal (set::difference (to-oset x)
+                          (to-oset y))
+         (to-oset (diff x y)))
+  :enable (to-oset
+           diff
+           fix
+           setp
+           empty))
+
+(add-to-ruleset from-oset-theory '(oset-difference-of-to-oset))
+
+(defrule from-oset-of-oset-difference
+  (equal (from-oset (set::difference x y))
+         (diff (from-oset x)
+               (from-oset y)))
+  :enable (double-containment
+           pick-a-point))
+
+(add-to-ruleset from-oset-theory '(from-oset-of-oset-difference))
+
+(defruled oset-difference-becomes-diff
+  (equal (set::difference x y)
+         (to-oset (diff (from-oset x)
+                        (from-oset y))))
+  :enable set::expensive-rules)
+
+(add-to-ruleset from-oset-theory '(oset-difference-becomes-diff))
+
+(defruled diff-becomes-oset-difference
+  (equal (diff x y)
+         (from-oset (set::difference (to-oset x)
+                                     (to-oset y)))))
+
+(add-to-ruleset to-oset-theory '(diff-becomes-oset-difference))
+
 ;;;;;;;;;;;;;;;;;;;;;;;;;;;;;;;;;;;;;;;;;;;;;;;;;;;;;;;;;;;;;;;;;;;;;;;;;;;;;;;;
 
 (define diff-=
@@ -136,9 +205,9 @@
    (y acl2-number-setp))
   (mbe :logic (diff x y)
        :exec (acl2-number-tree-diff x y))
-  :guard-hints (("Goal" :in-theory (enable setp
-                                           set-all-acl2-numberp
-                                           diff))))
+  :guard-hints (("Goal" :in-theory (enable* break-abstraction
+                                            set-all-acl2-numberp
+                                            diff))))
 
 ;;;;;;;;;;;;;;;;;;;;;;;;;;;;;;;;;;;;;;;;
 
@@ -147,9 +216,9 @@
    (y symbol-setp))
   (mbe :logic (diff x y)
        :exec (symbol-tree-diff x y))
-  :guard-hints (("Goal" :in-theory (enable setp
-                                           set-all-symbolp
-                                           diff))))
+  :guard-hints (("Goal" :in-theory (enable* break-abstraction
+                                            set-all-symbolp
+                                            diff))))
 
 ;;;;;;;;;;;;;;;;;;;;;;;;;;;;;;;;;;;;;;;;
 
@@ -158,6 +227,6 @@
    (y eqlable-setp))
   (mbe :logic (diff x y)
        :exec (eqlable-tree-diff x y))
-  :guard-hints (("Goal" :in-theory (enable setp
-                                           set-all-eqlablep
-                                           diff))))
+  :guard-hints (("Goal" :in-theory (enable* break-abstraction
+                                            set-all-eqlablep
+                                            diff))))
